Syntax.thy
@@ -4,21 +4,25 @@ begin
 
 chapter \<open>While Language Syntax\<close>
 
-text \<open>A While language with non-deterministic choice, iteration and parallel composition.\<close>
-datatype 'a com =
+text \<open>
+A While language with non-deterministic choice, iteration and parallel composition.
+Also includes special commands for environment steps, which is useful for describing
+refinement properties. These have no evaluation semantics or rules however.
+\<close>
+datatype ('a,'b) com =
   Nil
-  | Abort
+  | Env "'b rel"
   | Basic "'a"
-  | Seq "'a com" "'a com" (infixr ";;" 80)
-  | Choice "'a com" "'a com" (infixr "\<sqinter>" 150)
-  | Loop "'a com" ("_*" [100] 150)
-  | Parallel "'a com" "'a com"  (infixr "||" 150)
+  | Seq "('a,'b) com" "('a,'b) com" (infixr ";" 80)
+  | Choice "('a,'b) com" "('a,'b) com" (infixr "\<sqinter>" 150)
+  | Loop "('a,'b) com" ("_*" [100] 150)
+  | Parallel "('a,'b) com" "('a,'b) com"  (infixr "||" 150)
 
 text \<open>Ensure there is no parallelism within a program\<close>
-fun local :: "'a com \<Rightarrow> bool"
+fun local :: "('a,'b) com \<Rightarrow> bool"
   where 
     "local (c\<^sub>1 || c\<^sub>2) = False" |
-    "local (c\<^sub>1 ;; c\<^sub>2) = (local c\<^sub>1 \<and> local c\<^sub>2)" |    
+    "local (c\<^sub>1 ; c\<^sub>2) = (local c\<^sub>1 \<and> local c\<^sub>2)" |    
     "local (c\<^sub>1 \<sqinter> c\<^sub>2) = (local c\<^sub>1 \<and> local c\<^sub>2)" |  
     "local (c*) = (local c)" |    
     "local _ = True"
